Tests/FBoundV2Spec.lean
@@ -1,0 +1,36 @@
+import «Lp2lc».Active.Util
+
+namespace Tests.FBoundV2Spec
+
+open Lp2lc.Active.Util
+
+def group : FBoundGroup Nat Nat where
+  save := id
+  load := id
+  roundtrip := by
+    intro value
+    rfl
+
+@[reducible] def boolMetadata : FBoundV2 group (λ _value => Bool) where
+  loadMetadata := λ _id => false
+
+@[reducible] def unitMetadata : FBoundV2 group (λ _value => Unit) where
+  loadMetadata := λ _id => ()
+
+section save
+
+example :
+    boolMetadata.save ⟨1, true⟩ = boolMetadata.save ⟨1, false⟩ := by
+  rfl
+
+example :
+    boolMetadata.save ⟨1, true⟩ = unitMetadata.save ⟨1, ()⟩ := by
+  rfl
+
+example :
+    (boolMetadata.load (boolMetadata.save ⟨1, true⟩)).fst = 1 := by
+  rfl
+
+end save
+
+end Tests.FBoundV2Spec
